extend shallow embedding
for array and loop functions

isa/CogentCommon_common_Tuples.thy
@@ -2,24 +2,110 @@ theory CogentCommon_common_Tuples
   imports "ShallowShared_Tuples"
 begin
 
+text \<open>Iteration Functions\<close>
+
+text \<open>Auxiliary functions:
+      seq32_cnt is used to calculate the number of intended iterations from start, end and step values. 
+      seq32_term is used as premise for termination. 
+        Even if the end value is specified, due to word arithmetic the loop counter could overflow in the
+        last step and start again. (This can only happen if the step is not 1). 
+        We use a simplified condition here, which is slightly stronger than necessary.
+        Another reason for non-termination would be if step is 0 (which is not tested in the C implementation
+        of seq32_simple).\<close>
+
+definition seq32_cnt :: "32 word \<Rightarrow> 32 word \<Rightarrow> 32 word \<Rightarrow> nat" where
+  "seq32_cnt frm to step \<equiv> ((unat to)-(unat frm)+(unat step)-1) div (unat step)"
+
+definition seq32_term :: "32 word \<Rightarrow> 32 word \<Rightarrow> bool" where 
+  "seq32_term to step \<equiv> (step > 0) \<and> ((unat to) + (unat step) \<le> 2 ^ LENGTH(32))"
+
+text \<open>seq32_simple\<close>
+
+text \<open>As basic implementation we use a recursive function which counts from 0 in steps of 1.\<close>
 fun seq32_simple_imp :: "nat \<Rightarrow> ('acc \<Rightarrow> 'acc) \<Rightarrow> 'acc \<Rightarrow> 'acc" where
-    "seq32_simple_imp cnt f acc = 
-      (if cnt = 0 then acc 
-       else seq32_simple_imp (cnt-1) f (f acc))"
+    "seq32_simple_imp 0 f acc = acc" |
+    "seq32_simple_imp (Suc n) f acc = f (seq32_simple_imp n f acc)"
 
-axiomatization where seq32_simple_def[simp]: 
-  "\<And>(acc::'acc) (f::'acc \<Rightarrow> 'acc). step \<noteq> 0 \<Longrightarrow> seq32_simple (Seq32SimpleParam.make frm to step f acc) = seq32_simple_imp (unat ((to - frm + step) div step)) f acc"
+text \<open>Function seq32_simple is defined by reduction to seq32_simple_imp.\<close>
+axiomatization where seq32_simple_def: 
+  "\<And>(acc::'acc) (f::'acc \<Rightarrow> 'acc). seq32_term to step \<Longrightarrow> 
+     seq32_simple \<lparr>Seq32SimpleParam.frm\<^sub>f=frm, to\<^sub>f=to, step\<^sub>f=step, f\<^sub>f=f, acc\<^sub>f=acc\<rparr> \<equiv> 
+       seq32_simple_imp (seq32_cnt frm to step) f acc"
 
-fun seq32_imp :: "nat \<Rightarrow> 32 word \<Rightarrow> 32 word \<Rightarrow> ('acc, 'obsv, 'rbrk) Seq32_body \<Rightarrow> 'acc \<Rightarrow> 'obsv \<Rightarrow> ('acc, 'rbrk) LRR\<^sub>T" where
-  "seq32_imp cnt idx step f acc obsv = 
-    (if cnt = 0 then ( acc, Iterate ())
-     else let fres = f (Seq32_bodyParam.make acc obsv idx) 
-          in case snd fres of Break _ \<Rightarrow> fres
-             | Iterate() \<Rightarrow> seq32_imp (cnt-1) (idx+step) step f (fst fres) obsv)"
+text \<open>Induction rules for seq32_simple:\<close>
 
-axiomatization where seq32_step0[simp]: 
-  "\<And>(acc::'acc) (obsv::'obsv) (f::('acc, 'obsv, 'rbrk) Seq32_body) .seq32 (Seq32Param.make frm to 0 f acc obsv) = (acc, Iterate())"
-axiomatization where seq32_def[simp]: 
-  "\<And>(acc::'acc) (obsv::'obsv) (f::('acc, 'obsv, 'rbrk) Seq32_body) .step \<noteq> 0 \<Longrightarrow> seq32 (Seq32Param.make frm to step f acc obsv) = seq32_imp (unat ((to - frm + step) div step)) frm step f acc obsv"
+text \<open>The first induction rule is intended for properties P which do not depend on the current loop counter,
+      i.e., true loop invariants. For the induction step it must be proven than an every application of function
+      f preserves P.\<close>
+lemma seq32_simple_imp_induct_f: "(P acc) \<Longrightarrow> (\<And>a. (P a) \<Longrightarrow> (P (f a))) \<Longrightarrow> (P (seq32_simple_imp n f acc))"
+  by (induct n, auto)
+
+lemma seq32_simple_induct_f:
+  "seq32_term to step \<Longrightarrow> P(acc) \<Longrightarrow> (\<And>a. P(a) \<Longrightarrow> P(f(a))) \<Longrightarrow>
+   P(seq32_simple \<lparr>Seq32SimpleParam.frm\<^sub>f=frm, to\<^sub>f=to, step\<^sub>f=step, f\<^sub>f=f, acc\<^sub>f=acc \<rparr>)"
+  by(unfold seq32_simple_def, rule seq32_simple_imp_induct_f, auto)
+
+text \<open>The second induction rule is intended for properties P which additionally depend on the current loop counter.
+      For the induction step it must be proven that every application of function f preserves P for the incremented
+      loop counter. As additional induction premise the loop counter can be assumed to be lower than the overall
+      number of iterations in the final thesis.\<close>
+lemma seq32_simple_imp_induct: "(P 0 acc) \<Longrightarrow> (\<And>a i. i < n \<Longrightarrow> (P i a) \<Longrightarrow> (P (Suc i) (f a))) \<Longrightarrow> (P n (seq32_simple_imp n f acc))"
+  by (induct n, auto)
+
+lemma seq32_simple_induct:
+  "seq32_term to step \<Longrightarrow> (P 0 acc) \<Longrightarrow> (\<And>a i. i < (seq32_cnt frm to step) \<Longrightarrow> (P i a) \<Longrightarrow> (P (Suc i) (f a))) \<Longrightarrow>
+   (P (seq32_cnt frm to step) (seq32_simple \<lparr>Seq32SimpleParam.frm\<^sub>f=frm, to\<^sub>f=to, step\<^sub>f=step, f\<^sub>f=f, acc\<^sub>f=acc \<rparr>))"
+  by (unfold seq32_simple_def, rule seq32_simple_imp_induct, auto)
+
+text \<open>seq32\<close>
+
+text \<open>As basic implementation we use a recursive function which counts from 0 in steps of 1.
+      It takes the start, step, and obsv values as additional arguments for providing the arguments of the body function.\<close>
+fun seq32_imp :: "nat \<Rightarrow> ('acc, 'obsv, 'rbrk) Seq32_body \<Rightarrow> 'acc \<Rightarrow> 32 word \<Rightarrow> 32 word \<Rightarrow> 'obsv \<Rightarrow> ('acc, 'rbrk) LRR\<^sub>T" where
+    "seq32_imp 0 f acc frm step obsv = (acc, Iterate())" |
+    "seq32_imp (Suc n) f acc frm step obsv = 
+       (let (acc, lres) = seq32_imp n f acc frm step obsv
+        in case lres of
+          Break _ \<Rightarrow> (acc, lres) |
+          Iterate _ \<Rightarrow> f \<lparr>Seq32_bodyParam.acc\<^sub>f = acc, obsv\<^sub>f = obsv, idx\<^sub>f = frm + (of_nat n)*step \<rparr>)"
+
+text \<open>Function seq32 is defined by reduction to seq32_imp.\<close>
+axiomatization where seq32_def: 
+  "\<And>(acc::'acc) (obsv::'obsv) (f::('acc, 'obsv, 'rbrk) Seq32_body). seq32_term to step \<Longrightarrow> 
+     seq32 \<lparr>Seq32Param.frm\<^sub>f=frm, to\<^sub>f=to, step\<^sub>f=step, f\<^sub>f=f, acc\<^sub>f=acc, obsv\<^sub>f=obsv\<rparr> \<equiv> 
+       seq32_imp (seq32_cnt frm to step) f acc frm step obsv"
+
+text \<open>The induction rule is intended for properties P which additionally depend on the current loop counter and the observed term.
+      The induction step consists of two parts for the cases Iterate and Break.
+      For the first case it must be proven that every application of function f preserves P for the incremented
+      loop counter. For the second case it must be proven that P holds for the incremented loop counter.
+      As additional induction premise the loop counter can be assumed to be lower than the overall
+      number of iterations in the final thesis.\<close>
+
+lemma seq32_imp_induct:
+  "P 0 (acc, Iterate()) obsv \<Longrightarrow> 
+   (\<And>a i r. i < n \<Longrightarrow> 
+      (P i (a,Iterate()) obsv \<longrightarrow> 
+           P (Suc i) (f \<lparr>Seq32_bodyParam.acc\<^sub>f=a, obsv\<^sub>f=obsv, idx\<^sub>f=frm+(of_nat i)*step\<rparr>) obsv)
+    \<and> (P i (a,Break r) obsv \<longrightarrow> P (Suc i) (a,Break r) obsv)) \<Longrightarrow> 
+   P n (seq32_imp n f acc frm step obsv) obsv"
+  apply(induct n)
+   apply(simp add:split_def)
+  apply(case_tac "seq32_imp n f acc frm step obsv")
+  apply(case_tac b)
+  by auto
+
+lemma seq32_induct:   
+  "seq32_term to step \<Longrightarrow> 
+   P 0 (acc,Iterate()) obsv \<Longrightarrow> 
+   (\<And>a i r. i < (seq32_cnt frm to step) \<Longrightarrow> 
+       (P i (a,Iterate()) obsv \<longrightarrow>
+           P (Suc i) (f \<lparr>Seq32_bodyParam.acc\<^sub>f=a, obsv\<^sub>f = obsv, idx\<^sub>f=frm+(of_nat i)*step \<rparr>) obsv)
+     \<and> (P i (a,Break r) obsv \<longrightarrow> P (Suc i) (a,Break r) obsv)) \<Longrightarrow>
+   P (seq32_cnt frm to step) (seq32 \<lparr>Seq32Param.frm\<^sub>f=frm, to\<^sub>f=to, step\<^sub>f=step, f\<^sub>f=f, acc\<^sub>f=acc, obsv\<^sub>f = obsv \<rparr>) obsv"
+  for f::"('acc, 'obsv, 'rbrk) Seq32_body" and acc::'acc and obsv::'obsv
+  apply(unfold seq32_def)
+  apply(rule_tac P=P  in seq32_imp_induct)
+  by auto
 
 end
