isa/Gencot_CArray_Tuples.thy
@@ -3,57 +3,159 @@ theory Gencot_CArray_Tuples
     Gencot_Default_Tuples
 begin
 
-text \<open>First we define the array functions for fixed lists\<close>
+text \<open>Define the array functions for fixed lists\<close>
 
-definition getArr' :: "('n::finite, 'el) FixedList \<Rightarrow> 32 word \<Rightarrow> 'el"
+definition getArr' :: "('n::len, 'el) FixedList \<Rightarrow> 'idx::len word \<Rightarrow> 'el"
   where 
     "getArr' lst idx \<equiv>
-      if unat idx >= CARD('n) then hd (Rep_FixedList lst)
+      if unat idx >= LENGTH('n) then hd (Rep_FixedList lst)
       else (nth (Rep_FixedList lst) (unat idx))"
 
-definition setArr' :: "('n::finite, 'el) FixedList \<Rightarrow> 32 word \<Rightarrow> 'el \<Rightarrow> ('n, 'el) FixedList"
+definition setArr' :: "('n::len, 'el) FixedList \<Rightarrow> 'idx::len word \<Rightarrow> 'el \<Rightarrow> ('n, 'el) FixedList"
   where
     "setArr' lst idx elm \<equiv> 
-      if unat idx >= CARD('n) then lst
+      if unat idx >= LENGTH('n) then lst
       else (Abs_FixedList (list_update (Rep_FixedList lst) (unat idx) elm))"
 
-definition modifyArr' :: "('n::finite, 'el) FixedList \<Rightarrow> 32 word \<Rightarrow> ('el \<times> 'arg \<Rightarrow> 'el \<times> 'arg) \<Rightarrow> 'arg \<Rightarrow> ('n, 'el) FixedList \<times> 'arg"
+definition modifyArr' :: "('n::len, 'el) FixedList \<Rightarrow> 'idx::len word \<Rightarrow> ('el \<times> 'arg \<Rightarrow> 'el \<times> 'arg) \<Rightarrow> 'arg \<Rightarrow> ('n, 'el) FixedList \<times> 'arg"
   where
     "modifyArr' lst idx chf inp \<equiv> 
-      if unat idx >= CARD('n) then (lst, inp)
+      if unat idx >= LENGTH('n) then (lst, inp)
       else let l = Rep_FixedList lst; elm = nth l (unat idx); chres = chf(elm, inp)
         in (Abs_FixedList (list_update l (unat idx) (fst chres)), snd chres)"
 
-definition modifyArrDflt' :: "('n::finite, 'el) FixedList \<Rightarrow> 32 word \<Rightarrow> ('el \<times> 'arg \<Rightarrow> 'el \<times> 'out) \<Rightarrow> 'arg \<Rightarrow> ('n, 'el) FixedList \<times> 'out"
+definition modifyArrDflt' :: "('n::len, 'el) FixedList \<Rightarrow> 'idx::len word \<Rightarrow> ('el \<times> 'arg \<Rightarrow> 'el \<times> 'out) \<Rightarrow> 'arg \<Rightarrow> ('n, 'el) FixedList \<times> 'out"
   where
     "modifyArrDflt' lst idx chf inp \<equiv> 
-      if unat idx >= CARD('n) then (lst, defaultVal ())
+      if unat idx >= LENGTH('n) then (lst, defaultVal ())
       else let l = Rep_FixedList lst; elm = nth l (unat idx); chres = chf(elm, inp)
         in (Abs_FixedList (list_update l (unat idx) (fst chres)), snd chres)"
 
-text \<open>
-  This locale has the wrapper record access and constructor as parameters.
-  It defines the array functions for the wrapper record and proves some useful lemmas.\<close>
+text \<open>Lift arrays to the wrapper records.
+      We introduce an overloaded abstract data type for all such arrays with indexes of type nat.
+      It consists of the following functions.
+      Array accesses are always guarded by function vld.\<close>
+consts 
+  siz :: "'arr \<Rightarrow> nat"
+  vld :: "'arr \<Rightarrow> nat \<Rightarrow> bool"
+  elm :: "'arr \<Rightarrow> nat \<Rightarrow> 'el"
+  upd :: "'arr \<Rightarrow> nat \<Rightarrow> 'el \<Rightarrow> 'arr"
 
-locale CArrFuns = fixes fld :: "'arr \<Rightarrow> ('n::finite, 'el) FixedList" and wrp :: "('n, 'el) FixedList \<Rightarrow> 'arr"
+text \<open>For every actual wrapper record the following locale will be interpreted.
+      It takes the wrapper record access and constructor as parameters.
+      The locale defines the laws of the abstract data type, 
+      specific array functions for the wrapper record and their conversion to the abstract data type functions.\<close>
+
+locale CArrFuns = 
+  fixes 
+    fld :: "'arr \<Rightarrow> ('n::len, 'el) FixedList" and 
+    wrp :: "('n, 'el) FixedList \<Rightarrow> 'arr"
+  assumes 
+    fld_inverse: "\<And>x. wrp (fld x) = x" and 
+    wrp_inverse: "\<And>x. fld (wrp x) = x" 
 begin
-definition getArrFxd :: "'arr \<times> 32 word \<Rightarrow> 'el"
+text \<open>Lift the array functions from fixed lists to the wrapper record.\<close>
+definition getArrFxd :: "'arr \<times> ('m::len) word \<Rightarrow> 'el"
   where "getArrFxd arg \<equiv> let (arr,idx) = arg in getArr' (fld arr) idx"
-definition setArrFxd :: "'arr \<times> 32 word \<times> 'el \<Rightarrow> 'arr \<times> unit"
+definition setArrFxd :: "'arr \<times> ('m::len) word \<times> 'el \<Rightarrow> 'arr \<times> unit"
   where "setArrFxd arg \<equiv> let (arr,idx,elm) = arg in (wrp(setArr' (fld arr) idx elm), ())"
-definition modifyArrFxd :: "'arr \<times> 32 word \<times> ('el \<times> 'arg \<Rightarrow> 'el \<times> 'arg) \<times> 'arg \<Rightarrow> 'arr \<times> 'arg"
+definition modifyArrFxd :: "'arr \<times> ('m::len) word \<times> ('el \<times> 'arg \<Rightarrow> 'el \<times> 'arg) \<times> 'arg \<Rightarrow> 'arr \<times> 'arg"
   where "modifyArrFxd arg \<equiv> let (arr, idx, chf, inp) = arg; 
     (reslst,res) = modifyArr' (fld arr) idx chf inp in (wrp reslst, res)"
-definition modifyArrDfltFxd :: "'arr \<times> 32 word \<times> ('el \<times> 'arg \<Rightarrow> 'el \<times> 'out) \<times> 'arg \<Rightarrow> 'arr \<times> 'out"
+definition modifyArrDfltFxd :: "'arr \<times> ('m::len) word \<times> ('el \<times> 'arg \<Rightarrow> 'el \<times> 'out) \<times> 'arg \<Rightarrow> 'arr \<times> 'out"
   where "modifyArrDfltFxd arg \<equiv> let (arr, idx, chf, inp) = arg;
     (reslst,res) = modifyArrDflt' (fld arr) idx chf inp in (wrp reslst, res)"
 
+text \<open>Define conversion functions between lists and the wrapper record.\<close>
+definition lstFxd :: "'arr \<Rightarrow> 'el list"
+  where "lstFxd a \<equiv> Rep_FixedList (fld a)"
+definition arrFxd :: "'el list \<Rightarrow> 'arr"
+  where "arrFxd a \<equiv> wrp (Abs_FixedList a)"
+
+text \<open>Define the abstract data type functions for the wrapper record.\<close>
+definition sizFxd :: "'arr \<Rightarrow> nat"
+  where "sizFxd a \<equiv> length (lstFxd a)"
+definition vldFxd :: "'arr => nat => bool"
+  where "vldFxd a i \<equiv> i < sizFxd a"
+definition elmFxd :: "'arr \<Rightarrow> nat \<Rightarrow> 'el"
+  where "elmFxd a i \<equiv> nth (lstFxd a) i"
+definition updFxd :: "'arr \<Rightarrow> nat \<Rightarrow> 'el \<Rightarrow> 'arr"
+  where "updFxd a i e \<equiv> arrFxd (list_update (lstFxd a) i e)"
+
 text \<open>Arrays are never empty.\<close>
-lemma arrNotNil: "\<forall>x::'arr .  (Rep_FixedList (fld  x)) \<noteq> []"
+lemma arrNotNil: "\<forall>x::'arr .  lstFxd x \<noteq> []"
   apply(rule allI)
-  apply(cut_tac x = "(fld (x::'arr))" for el in Rep_FixedList )
+  apply(unfold lstFxd_def)
+  apply(cut_tac x = "(fld x)" in Rep_FixedList )
+  by auto
+
+text \<open>Laws for the abstract data type functions\<close>
+lemma sizArr: "sizFxd a = LENGTH('n)"
+  apply(unfold sizFxd_def lstFxd_def)
+  by (simp add: length_FixedList)
+lemma vldArr: "vldFxd a n = (n < LENGTH('n))"
+  by (simp add: vldFxd_def sizArr)
+lemma updArr: "vldFxd a i \<Longrightarrow> elmFxd (updFxd a i e) i = e"
+  apply(auto simp add: updFxd_def elmFxd_def lstFxd_def arrFxd_def wrp_inverse vldArr)
+  apply(subst Abs_FixedList_inverse)
+  apply(cut_tac x = "(fld a)" in Rep_FixedList )
   apply(auto)
+  apply(cut_tac x = "(fld a)" in Rep_FixedList )
+  by auto
+lemma updArrFrame: "vldFxd a i \<and> vldFxd a j \<and> i \<noteq> j \<Longrightarrow> elmFxd (updFxd a i e) j = elmFxd a j"
+  apply(auto simp add: updFxd_def elmFxd_def lstFxd_def arrFxd_def wrp_inverse vldArr)
+  apply(subst Abs_FixedList_inverse)
+  apply(cut_tac x = "(fld a)" in Rep_FixedList )
+  by (auto)
+
+text \<open>Array equality by extensionality. \<close>
+lemma eqArr1: "(\<And> i. (vldFxd a1 i) \<Longrightarrow> ((elmFxd a1 i) = (elmFxd a2 i))) \<Longrightarrow> (a1 = a2)"
+  apply(auto simp add: elmFxd_def vldFxd_def sizFxd_def lstFxd_def)
+  apply(drule nth_equalityI[rotated])
+  apply(cut_tac x = "(fld a1)" in Rep_FixedList )
+  apply(cut_tac x = "(fld a2)" in Rep_FixedList )
+  apply(simp)
+  apply(drule arg_cong[where f = Abs_FixedList])
+  apply(subst (asm) Rep_FixedList_inverse)+
+  apply(drule arg_cong[where f = wrp])
+  apply(simp add: fld_inverse)
   done
+lemma eqArr: "(a1 = a2) = (\<forall> i. (vldFxd a1 i) \<longrightarrow> ((elmFxd a1 i) = (elmFxd a2 i)))"
+  apply(rule iffI)
+   apply(rule allI)
+   apply(rule impI)
+   apply(auto)
+  by (rule eqArr1,auto)
+
+text \<open>Conversion laws for the array functions to the abstract data type.\<close>
+text \<open>Conversion for getArr\<close>
+lemma getArrValid: "vldFxd a (unat i) \<Longrightarrow> getArrFxd (a,i) = elmFxd a (unat i)"
+  by (simp add: getArrFxd_def getArr'_def vldArr elmFxd_def lstFxd_def)
+lemma getArrInvalid: "\<not> vldFxd a (unat i) \<Longrightarrow> getArrFxd (a,i) = elmFxd a 0"
+  apply(simp add: getArrFxd_def getArr'_def vldArr elmFxd_def)
+  apply(fold lstFxd_def)
+  apply(case_tac " lstFxd a")
+   apply(cut_tac arrNotNil)
+  by auto
+
+text \<open>Conversion for setArr\<close>
+lemma setArrValid: "vldFxd a (unat i) \<Longrightarrow> setArrFxd (a,i,v) = (updFxd a (unat i) v, ())"
+  by (simp add: setArrFxd_def setArr'_def vldArr lstFxd_def arrFxd_def updFxd_def)
+lemma setArrInvalid: "\<not> vldFxd a (unat i) \<Longrightarrow> setArrFxd (a,i,v) = (a,())"
+  by (simp add: setArrFxd_def setArr'_def vldArr fld_inverse)
+
+text \<open>Conversion for modifyArr\<close>
+lemma modifyArrValid: "vldFxd a (unat i) \<Longrightarrow> modifyArrFxd (a,i,f,x) = (let (e,y) = f (elmFxd a (unat i), x) in (updFxd a (unat i) e, y))"
+  by (simp add: modifyArrFxd_def modifyArr'_def split_def Let_def vldArr lstFxd_def arrFxd_def updFxd_def elmFxd_def)
+lemma modifyArrInvalid: "\<not> (vldFxd a (unat i))  ==> modifyArrFxd (a,i,f,x) = (a, x)"
+  by (simp add: modifyArrFxd_def modifyArr'_def vldArr fld_inverse)
+
+text \<open>Conversion for modifyArrDfl\<close>
+lemma modifyArrDfltValid: "vldFxd a (unat i)   ==> modifyArrDfltFxd (a,i,f,x) = (let (e,y) = f (elmFxd a (unat i), x) in (updFxd a (unat i) e, y))"
+  by (simp add: modifyArrDfltFxd_def modifyArrDflt'_def split_def Let_def vldArr lstFxd_def arrFxd_def updFxd_def elmFxd_def)
+lemma modifyArrDfltInvalid: "\<not> (vldFxd a (unat i))  ==> modifyArrDfltFxd (a,i,f,x) = (a, defaultVal ())"
+  by (simp add: modifyArrDfltFxd_def modifyArrDflt'_def vldArr fld_inverse)
+
 end
 
 end
