isa/GencotTypes.thy
@@ -1,18 +1,15 @@
 theory GencotTypes
-  imports "HOL-Library.Numeral_Type"
+  imports "HOL-Library.Type_Length"
 begin
 
 text \<open>The type of lists with a fixed length, used for representing C arrays\<close>
 
-typedef ('n::finite, 'a) FixedList =  "{x::'a list. length x = CARD('n)}"
-apply (rule_tac x = "replicate CARD('n) (_::'a)" in exI)
+typedef (overloaded) ('n::len, 'a) FixedList =  "{x::'a list. length x = LENGTH('n)}"
+  apply (rule_tac x = "replicate LENGTH('n) (_::'a)" in exI)
   by simp
 
-text \<open>
-  Type MayNull is represented using HOL.option. 
-  Since Cogent common also defines a type Option with the same variants,
-  we make the HOL.option variant names available by alias names.\<close>
-abbreviation HOLSome where "HOLSome \<equiv> Some"
-abbreviation HOLNone where "HOLNone \<equiv> None"
+lemma length_FixedList: "length (Rep_FixedList x) = LENGTH('n)" for x::"('n::len, 'a) FixedList"
+  apply(insert Rep_FixedList)
+  by auto
 
 end
