isa/Gencot_MayNull_Tuples.thy
@@ -2,9 +2,9 @@ theory Gencot_MayNull_Tuples
   imports ShallowShared_Tuples
 begin
 
-axiomatization where null_def[simp]: "null () = HOLNone" 
-axiomatization where mayNull_def[simp]: "\<forall>x . mayNull x = HOLSome x" 
-axiomatization where notNull_def[simp]: "\<forall>x . notNull x = (case x of HOLNone \<Rightarrow> None () | HOLSome y \<Rightarrow> Some y)" 
-axiomatization where roNotNull_def[simp]: "\<forall>x . roNotNull x = (case x of HOLNone \<Rightarrow> None () | HOLSome y \<Rightarrow> Some y)" 
+axiomatization where null_def[simp]: "null () = option.None" 
+axiomatization where mayNull_def[simp]: "\<forall>x . mayNull x = option.Some x" 
+axiomatization where notNull_def[simp]: "\<forall>x . notNull x = (case x of option.None \<Rightarrow> None () | option.Some y \<Rightarrow> Some y)" 
+axiomatization where roNotNull_def[simp]: "\<forall>x . roNotNull x = (case x of option.None \<Rightarrow> None () | option.Some y \<Rightarrow> Some y)" 
 
 end
